progs/conclib.v
@@ -3091,32 +3091,52 @@ eapply (semax_fun_id'' _f); try reflexivity.
 
 (* revised start_function that mostly works for dependent specs *)
 Ltac start_dep_function := 
-  match goal with |- semax_body ?V ?G ?F ?spec =>
+ leaf_function;
+ match goal with |- semax_body _ _ ?F ?spec =>
+   let D := constr:(type_of_function F) in 
+   let S := constr:(type_of_funspec (snd spec)) in
+   let D := eval hnf in D in let D := eval simpl in D in 
+   let S := eval hnf in S in let S := eval simpl in S in 
+   tryif (unify D S) then idtac else
+   tryif function_types_compatible D S 
+   then idtac "Warning: the function-body parameter/return types are not identical to the funspec types, although they are compatible:
+Function body:" D "
+Function spec:" S
+   else
+   (fail "Function signature (param types, return type) from function-body does not match function signature from funspec
+Function body: " D "
+Function spec: " S);
+   check_normalized F
+ end;
+ match goal with |- semax_body ?V ?G ?F ?spec =>
     let s := fresh "spec" in
-    pose (s:=spec); hnf in s;
+    pose (s:=spec); hnf in s; simpl in s;
     match goal with
-    | s :=  (DECLARE _ WITH _ : globals
+    | s :=  (DECLARE _ WITH _: globals
                PRE  [] main_pre _ nil _
-               POST [ tint ] main_post _ nil _) |- _ => idtac
+               POST [ tint ] _) |- _ => idtac
     | s := ?spec' |- _ => check_canonical_funspec spec'
    end;
    change (semax_body V G F s); subst s
  end;
  let DependedTypeList := fresh "DependedTypeList" in
  match goal with |- semax_body _ _ _ (pair _ (mk_funspec _ _ _ ?Pre _ _ _)) =>
-   match Pre with 
-   | (fun x => match _ with (a,b) => _ end) => intros Espec DependedTypeList [a b] 
+   match Pre with
+   | (fun x => match _ with (a,b) => _ end) => intros Espec DependedTypeList [a b]
    | (fun i => _) => intros Espec DependedTypeList i
    end;
    simpl fn_body; simpl fn_params; simpl fn_return
  end;
  simpl functors.MixVariantFunctor._functor in *;
  simpl rmaps.dependent_type_functor_rec;
- repeat match goal with |- @semax _ _ _ (match ?p with (a,b) => _ end * _) _ _ =>
+ clear DependedTypeList;
+ repeat match goal with | |- @semax _ _ _ (match ?p with (a,b) => _ end * _) _ _ =>
+             destruct p as [a b]
+                                          | |- @semax _ _ _ ((match ?p with (a,b) => _ end) eq_refl * _) _ _ =>
              destruct p as [a b]
            end;
  simplify_func_tycontext;
- repeat match goal with 
+ repeat match goal with
  | |- context [Sloop (Ssequence (Sifthenelse ?e Sskip Sbreak) ?s) Sskip] =>
        fold (Swhile e s)
  | |- context [Ssequence ?s1 (Sloop (Ssequence (Sifthenelse ?e Sskip Sbreak) ?s2) ?s3) ] =>
@@ -3131,12 +3151,12 @@ Ltac start_dep_function :=
                                   but it needs to come after process_stackframe_of *)
  repeat rewrite <- data_at__offset_zero;
  try apply start_function_aux1;
- repeat (apply semax_extract_PROP; 
+ repeat (apply semax_extract_PROP;
               match goal with
               | |- _ ?sh -> _ =>
                  match type of sh with
-                 | share => intros ?SH 
-                 | Share.t => intros ?SH 
+                 | share => intros ?SH
+                 | Share.t => intros ?SH
                  | _ => intro
                  end
                | |- _ => intro
@@ -3144,7 +3164,15 @@ Ltac start_dep_function :=
  first [ eapply eliminate_extra_return'; [ reflexivity | reflexivity | ]
         | eapply eliminate_extra_return; [ reflexivity | reflexivity | ]
         | idtac];
- abbreviate_semax.
+ abbreviate_semax;
+ lazymatch goal with 
+ | |- semax ?Delta (PROPx _ (LOCALx ?L _)) _ _ => check_parameter_vals Delta L
+ | _ => idtac
+ end;
+ try match goal with DS := @abbreviate (PTree.t funspec) PTree.Leaf |- _ =>
+     clearbody DS
+ end;
+ start_function_hint.
 
 (* Notations for dependent funspecs *)
 Notation "'TYPE' A 'WITH'  x1 : t1 , x2 : t2 'PRE'  [ u , .. , v ] P 'POST' [ tz ] Q" :=
